almost done no Free var

Lambda.dfy
@@ -2,13 +2,12 @@ include "objects.dfy"
 type Id= nat
 datatype LambdaTerm = Var(id:Id) | Lambda(x:Id,t:LambdaTerm) | Application( t1:LambdaTerm, t2:LambdaTerm)
 
-function bound(t:LambdaTerm):seq<Id>
-    ensures allUnique(bound(t))
+function bound(t:LambdaTerm):set<Id>
 {
         match t
-                case Var(_) => []
-                case Lambda(x,t) => addition(x,bound(t))
-                case Application(t1,t2) => reunion(bound(t1),bound(t2))
+                case Var(_) => {}
+                case Lambda(x,t) => {x}+bound(t)
+                case Application(t1,t2) => bound(t1)+bound(t2)
 }
 predicate includes(s1:seq<Id>,s2:seq<Id>)
     
@@ -153,13 +152,12 @@ function remove(s:seq<Id>,x:Id):seq<Id>
 
 }
 
-function free(t:LambdaTerm):seq<Id>
-    ensures allUnique(free(t))
+function free(t:LambdaTerm):set<Id>
 {
      match t
-                case Var(x) => [x]
-                case Lambda(x,t) => remove(free(t),x)
-                case Application(t1,t2) => reunion(free(t1),free(t2))
+                case Var(x) => {x}
+                case Lambda(x,t) => free(t)-{x}
+                case Application(t1,t2) => free(t1)+free(t2)
 }
 
 function vars(t:LambdaTerm):seq<Id>
@@ -353,7 +351,6 @@ lemma CaSubstitution'OfVarDoesNotChangeHeight(t1:LambdaTerm, x:Id, t2:LambdaTerm
             } else if !(y in free(t2)) {
                 CaSubstitution'OfVarDoesNotChangeHeight(t1', x, t2, ids);
             } else {
-                // alpha-rename branch
                 var ids' := addAnUniqueId(ids);
                 var vari  := Var(ids'[0]);
                 var t2' := substitution(t1', y, vari);
@@ -402,6 +399,14 @@ predicate alphaEquivalence(t1:LambdaTerm,t2:LambdaTerm)
     alphaEquivalence'(t1,t2,[],[])
 }
 function findId(ids:seq<Id>,id:Id):Option<nat>
+    ensures !(id in ids) <==> findId(ids,id)==None 
+    ensures (id in ids) <==> findId(ids,id)!=None
+    ensures (id in ids) <==> var pos:|findId(ids,id)==Some(pos);
+    pos<|ids| && ids[pos]==id &&
+    (forall pos2:nat:: pos<pos2<|ids| ==> ids[pos2]!=id)
+    && 
+    forall pos3:nat:: (pos3<|ids| && ids[pos3]==id ) ==> pos3<=pos
+
     decreases ids
 {
     if ids==[] then None 
@@ -440,3 +445,340 @@ predicate alphaEquivalence'(t1:LambdaTerm,t2:LambdaTerm,id1:seq<Id>,id2:seq<Id>)
                                         case _=>false
 }
 
+lemma EqualTermsAreAlphaEquilvalent(t1:LambdaTerm,t2:LambdaTerm)
+    requires t1==t2 
+    ensures alphaEquivalence(t1,t2)
+{
+    EqualTermsAreAlphaEquilvalent'(t1,t2,[],[]);
+}
+
+lemma EqualTermsAreAlphaEquilvalent'(t1:LambdaTerm,t2:LambdaTerm,id1:seq<Id>,id2:seq<Id>)
+    requires forall y :: y in vars(t1) ==> findId(id1, y) == findId(id2, y)
+    requires |id1|==|id2|
+    requires t1==t2 
+    ensures alphaEquivalence'(t1,t2,id1,id2)
+    decreases minim(lHeight(t1),lHeight(t2))
+{
+        match t1
+            case Var(x) => {
+                assert t1==t2;
+                var y:|t2==Var(y);
+                assert x==y;
+                var r1:=findId(id1,x);
+                var r2:=findId(id2,y);
+                assert r1==r2;
+                if (r1==None)
+                {
+                    assert x==y;
+                }
+                assert alphaEquivalence'(t1,t2,id1,id2);
+            }
+            case Lambda(x,t1') => {
+                var y,t2':|t2==Lambda(y,t2');
+                assert y==x && t2'==t1';
+                var id1':=id1+[x];
+                var id2':=id2+[y];
+                assert findId(id1',x)==Some(|id1'|-1);
+                assert findId(id1',x)==findId(id2',y);
+                EqualTermsAreAlphaEquilvalent'(t1',t2',id1+[x],id2+[y]);
+            }
+            case Application(t1',t1'') => {
+                var t2',t2'':|t2==Application(t2',t2'');
+                EqualTermsAreAlphaEquilvalent'(t1',t2',id1,id2);
+                EqualTermsAreAlphaEquilvalent'(t1'',t2'',id1,id2);
+            }
+}
+
+
+lemma SubstAlphaEquivalence (t:LambdaTerm,x:Id,x':Id)
+    requires !(x' in vars(t))
+    ensures alphaEquivalence(Lambda(x,t),Lambda(x',substitution(t,x,Var(x'))))
+{
+    assert []+[x]==[x] && []+[x']==[x'];
+    SubstAlphaEquivalence'(t, x, x',substitution(t,x,Var(x')), [x], [x']);
+}
+
+
+lemma SubstAlphaEquivalence'(t:LambdaTerm, x:Id, x':Id,t2:LambdaTerm, id1:seq<Id>, id2:seq<Id>)
+    requires |id1| == |id2| >0
+    requires !(x' in vars(t))
+    requires id1[0]==x && id2[0]==x'
+    requires forall i :: 0 <= i < |id1| ==>
+        (id1[i] == x <==> id2[i] == x') &&
+        (id1[i] != x ==> id1[i] == id2[i])
+    requires t2==substitution(t,x,Var(x'))
+    ensures alphaEquivalence'(t, t2, id1, id2)
+    decreases lHeight(t)
+{
+    match t 
+        case Application(t1a,t1b) =>
+        {
+            var t2a:=substitution(t1a,x,Var(x'));
+            var t2b:=substitution(t1b,x,Var(x'));
+            assert t2==Application(t2a,t2b);
+
+            SubstAlphaEquivalence'(t1a,x,x',t2a,id1,id2);
+            SubstAlphaEquivalence'(t1b,x,x',t2b,id1,id2);
+
+            assert alphaEquivalence'(t1a,t2a,id1,id2);
+            assert alphaEquivalence'(t1b,t2b,id1,id2);
+
+            assert alphaEquivalence'(t,t2,id1,id2);
+        }
+        case Lambda(z,t1') =>
+        {
+            if z==x
+            {
+                assert t2==t;
+                var id1' := id1+[x] ;
+                var id2' := id2+[x] ;
+                
+
+                forall y | y in vars(t1') ensures findId(id1', y) == findId(id2', y) {
+                    if y != x {
+                        assert y in vars(t);
+                        assert y != x'; 
+                    }
+                }
+                EqualTermsAreAlphaEquilvalent'(t1',t1',id1',id2');
+                assert alphaEquivalence'(t, t2, id1, id2);
+            }
+            else 
+            {
+                
+                var t2' := substitution(t1', x, Var(x'));
+                assert t2 == Lambda(z, t2');
+
+                var id1':=id1+[z];
+                var id2':=id2+[z];
+
+                SubstAlphaEquivalence'(t1',x,x',t2',id1',id2');
+
+                assert alphaEquivalence'(t1',t2',id1',id2');
+            }
+        }
+        case Var(z) =>
+        {
+            if (z==x)
+            {
+                assert t2==Var(x');
+                var r1:=findId(id1,x);
+                var r2:=findId(id2,x');
+                assert r1!=None;
+                
+                assert r1==r2;
+            }
+            else 
+            {
+                assert t2==t;
+                assert z!=x';
+            }
+        }
+}
+
+lemma AlphaEquivSymmetric(t1:LambdaTerm, t2:LambdaTerm)
+    requires alphaEquivalence(t1, t2)
+    ensures alphaEquivalence(t2, t1)
+{
+    AlphaEquivSymmetric'(t1,t2,[],[]);
+}
+lemma AlphaEquivSymmetric'(t1:LambdaTerm, t2:LambdaTerm,id1:seq<Id>,id2:seq<Id>)
+    requires alphaEquivalence'(t1, t2,id1,id2)
+    ensures alphaEquivalence'(t2, t1,id2,id1)
+{
+
+
+}
+
+lemma ApplicationEquivalence(t1a:LambdaTerm,t2a:LambdaTerm,t1b:LambdaTerm,t2b:LambdaTerm)
+    requires alphaEquivalence(t1a,t2a) && alphaEquivalence(t1b,t2b)
+    ensures alphaEquivalence(Application(t1a,t1b),Application(t2a,t2b))
+{
+
+}
+
+lemma AlphaEquivTransitive(t1:LambdaTerm, t2:LambdaTerm, t3:LambdaTerm)
+    requires alphaEquivalence(t1, t2)
+    requires alphaEquivalence(t2, t3)
+    ensures alphaEquivalence(t1, t3)
+{
+    AlphaEquivTransitive'(t1,t2,t3,[],[],[]);
+}
+lemma AlphaEquivTransitive'(t1:LambdaTerm, t2:LambdaTerm, t3:LambdaTerm,id1:seq<Id>,id2:seq<Id>,id3:seq<Id>)
+    requires alphaEquivalence'(t1, t2,id1,id2)
+    requires alphaEquivalence'(t2, t3,id2,id3)
+    ensures alphaEquivalence'(t1, t3,id1,id3)
+{
+    
+}
+
+lemma LambdaEquivalence(t1:LambdaTerm,t2:LambdaTerm,x1:Id,x2:Id)
+    requires alphaEquivalence(t1,t2)
+    requires !(x1 in free(t1)) && !(x2 in free(t2))
+    ensures alphaEquivalence(Lambda(x1,t1),Lambda(x2,t2))
+{
+    LambdaEquivalence'(t1,t2,x1,x2,[],[]);
+    assert [x1]==[x1]+[] && [x2]==[x2]+[];
+    assert alphaEquivalence'(t1,t2,[x1],[x2]);
+    assert [x1]==[]+[x1] && [x2]==[]+[x2];
+}
+
+lemma findId_prepend(ids: seq<Id>, x: Id, val: Id)
+    ensures findId([val] + ids, x) ==
+        match findId(ids, x) {
+            case Some(i) => Some(i + 1)
+            case None => if x == val then Some(0) else None
+        }
+{
+    if ids == [] {
+    } else {
+        var len := |ids|;
+        var prepended := [val] + ids;
+        
+        if ids[len-1] == x {
+            assert prepended[|prepended|-1] == x;
+        } else {
+            assert prepended[..|prepended|-1] == [val] + ids[..len-1];
+            findId_prepend(ids[..len-1], x, val);
+        }
+    }
+}
+
+lemma LambdaEquivalence'(t1:LambdaTerm,t2:LambdaTerm,x1:Id,x2:Id,id1:seq<Id>,id2:seq<Id>)
+    requires alphaEquivalence'(t1,t2,id1,id2)
+    requires x1 in free(t1) ==> x1 in id1  
+    requires x2 in free(t2) ==> x2 in id2
+    ensures alphaEquivalence'(t1,t2,[x1]+id1,[x2]+id2)
+{
+    match t1 
+        case Var(x) =>
+        {
+            var y: Id :| t2 == Var(y);
+            var r1 := findId(id1, x);
+            var r2 := findId(id2, y);
+            
+            var id1' := [x1] + id1;
+            var id2' := [x2] + id2;
+            var r1' := findId(id1', x);
+            var r2' := findId(id2', y);
+
+            findId_prepend(id1, x, x1);
+            findId_prepend(id2, y, x2);
+
+            if r1 == None
+            {
+                assert x==y;
+                
+                assert x!=x1; 
+                
+                assert y!=x2;
+
+                assert !(x in id1');
+                assert !(y in id2');
+
+                assert r1'==None;
+                assert r2'==None;
+            }
+            else 
+            {
+                var i1 :|r1==Some(i1);
+                assert r2==Some(i1); 
+
+                var new_pos:=i1+1;
+
+                assert id1'[new_pos]==x;
+                
+             
+
+                
+                assert r1'==Some(new_pos);
+
+                assert id2'[new_pos]==y;
+
+                assert r2' == Some(new_pos);
+    }
+        }
+        case Lambda(x,t1')=>
+        {
+            var y:nat,t2':LambdaTerm:|t2==Lambda(y,t2');
+            var id1':=id1+[x];
+            var id2':=id2+[y];
+            LambdaEquivalence'(t1',t2',x1,x2,id1',id2');
+            assert [x1]+id1+[x]==[x1]+id1';
+            assert [x2]+id2+[y]==[x2]+id2';
+
+        }
+        case Application(t1a,t1b)=>
+        {
+            var t2a:LambdaTerm,t2b:LambdaTerm:|t2==Application(t2a,t2b);
+            LambdaEquivalence'(t1a,t2a,x1,x2,id1,id2);
+            LambdaEquivalence'(t1b,t2b,x1,x2,id1,id2);
+
+        }
+}
+
+
+lemma AlphaCongruenceLambda(y:Id, t1:LambdaTerm, t2:LambdaTerm)
+    requires alphaEquivalence(t1, t2)
+    ensures alphaEquivalence(Lambda(y, t1), Lambda(y, t2))
+{
+    assert []+[y]==[y]==[y]+[];
+    AlphaCongruenceLambda'( t1, t2,y, [], []);
+}
+
+lemma AlphaCongruenceLambda'(t1:LambdaTerm, t2:LambdaTerm,y:Id, id1:seq<Id>, id2:seq<Id>)
+    requires alphaEquivalence'(t1, t2, id1, id2)
+    ensures alphaEquivalence'(t1, t2, [y]+id1, [y]+id2)
+    decreases minim(lHeight(t1), lHeight(t2))
+{
+    match t1 {
+        case Var(x) => {
+            var z :| t2 == Var(z);
+            var r1:=findId(id1, x);
+            var r2:=findId(id2, z);
+            
+            var id1':=[y]+id1;
+            var id2':=[y]+id2;
+            var r1':=findId(id1', x);
+            var r2':=findId(id2', z);
+
+            findId_prepend(id1, x, x);
+            findId_prepend(id2, y, x);
+
+            if r1 == None {
+                assert x == z;
+                if x == y {
+                    assert id1'[0] == x;
+                    assert r1' == Some(0);
+
+                    assert id2'[0] == z;
+                    assert r2' == Some(0);
+
+                } else {
+                    assert r1' == None;
+                    assert r2' == None;
+                }
+            } else {
+                var i1 :| r1 == Some(i1);
+                var new_pos := i1 + 1;
+
+                assert id1'[new_pos] == x;
+                assert r1' == Some(new_pos);
+
+                assert id2'[new_pos] == z;
+                assert r2' == Some(new_pos);
+            }
+        }
+        case Lambda(x, t1') => {
+            var z, t2' :| t2 == Lambda(z, t2');
+            AlphaCongruenceLambda'( t1', t2',y, id1+[x], id2+[z]);
+            assert [y]+id1+[x] == [y] + (id1+[x]);
+            assert [y]+id2+[z] == [y] + (id2+[z]);
+        }
+        case Application(t1a, t1b) => {
+            var t2a, t2b :| t2 == Application(t2a, t2b);
+            AlphaCongruenceLambda'( t1a, t2a,y, id1, id2);
+            AlphaCongruenceLambda'( t1b, t2b,y, id1, id2);
+        }
+    }
+}
